wip, copy MinimalMMIO because incompatible with Kami/riscv-coq proof,
still doesn't compile, and access_size.word depending on machine width
and being the same as access_size.four in case of 32bit causes trouble

investigations/bedrock2/LibBase/MMIOLabels.v
@@ -3,42 +3,49 @@
 Require Import Coq.Strings.String. Local Open Scope string_scope.
 Require Import bedrock2.Syntax.
 
-Definition READ_PREFIX := "READ".
+Definition READ_PREFIX := "MMIOREAD".
 Definition READ8 := READ_PREFIX ++ "8".
 Definition READ16 := READ_PREFIX ++ "16".
 Definition READ32 := READ_PREFIX ++ "32".
-Definition READW := READ_PREFIX ++ "W". (* read 32 or 64 bits depending on bitwidth of machine *)
+Definition READ64 := READ_PREFIX ++ "64".
 
-Definition WRITE_PREFIX := "WRITE".
+Definition WRITE_PREFIX := "MMIOWRITE".
 Definition WRITE8 := WRITE_PREFIX ++ "8".
 Definition WRITE16 := WRITE_PREFIX ++ "16".
 Definition WRITE32 := WRITE_PREFIX ++ "32".
-Definition WRITEW := WRITE_PREFIX ++ "W". (* write 32 or 64 bits depending on bitwidth of machine *)
+Definition WRITE64 := WRITE_PREFIX ++ "64".
 
-Definition access_size_to_MMIO_suffix(sz: access_size): string :=
+Require Import coqutil.Word.Interface.
+Require Import Coq.Numbers.DecimalString.
+Require Import Coq.ZArith.ZArith.
+
+Definition ZToStr(n: Z): string := DecimalString.NilZero.string_of_int (Z.to_int n).
+
+Definition access_size_to_MMIO_suffix(width: Z)(sz: access_size): string :=
   match sz with
   | access_size.one => "8"
   | access_size.two => "16"
   | access_size.four => "32"
-  | access_size.word => "W"
+  | access_size.word => ZToStr width
   end.
 
-Definition access_size_to_MMIO_read(sz: access_size): string :=
-  READ_PREFIX ++ access_size_to_MMIO_suffix sz.
+(* We pass an unnecessary `word` instance to the following definitions just to make
+   `width` inferrable, later we might make a typeclass for just `width` and then we
+   can remove the `word`. *)
+#[export] Hint Mode word.word - : typeclass_instances.
 
-Definition access_size_to_MMIO_write(sz: access_size): string :=
-  WRITE_PREFIX ++ access_size_to_MMIO_suffix sz.
+Definition access_size_to_MMIO_read{width}{word: word.word width}(sz: access_size): string :=
+  READ_PREFIX ++ access_size_to_MMIO_suffix width sz.
 
-Lemma access_size_to_MMIO_read_inj: forall sz1 sz2,
+Definition access_size_to_MMIO_write{width}{word: word.word width}(sz: access_size): string :=
+  WRITE_PREFIX ++ access_size_to_MMIO_suffix width sz.
+
+Lemma access_size_to_MMIO_read_inj{width}{word: word.word width}: forall sz1 sz2,
     access_size_to_MMIO_read sz1 = access_size_to_MMIO_read sz2 ->
     sz1 = sz2.
 Proof.
-  destruct sz1; destruct sz2; cbv; congruence.
-Qed.
-
-Lemma access_size_to_MMIO_write_inj: forall sz1 sz2,
-    access_size_to_MMIO_write sz1 = access_size_to_MMIO_write sz2 ->
-    sz1 = sz2.
-Proof.
-  destruct sz1; destruct sz2; cbv; congruence.
-Qed.
+  destruct sz1; destruct sz2; cbn; try congruence; intros.
+  3: {
+    inversion H.
+    (* doesn't hold!! *)
+Admitted.
