investigations/bedrock2/Riscv/MinimalMMIO.v
@@ -1,0 +1,322 @@
+(* Copied from riscv.Platform.MinimalMMIO, but adapted to log how many bits were
+   MMIO'd, which makes it incompatible with the Kami processor, whose connection
+   proof to riscv would take some time to update.
+   Also, should the trace contain zero-extended or sign-extended values?
+   Ideally, it would only contain the number of bytes read/written rather than a
+   whole word, but that's not compatible with how everything is set up.
+   Sign-extending depending on whether Lb or Lbu was used doesn't make sense
+   because that's not visible to the device, Lb vs Lbu only affects what the
+   processor does after obtaining the value, when placing it in a register.
+   So we choose to zero-extend in this file. *)
+Require Import Coq.Strings.String.
+Require Import Coq.Numbers.DecimalString.
+Require Import Coq.ZArith.ZArith.
+Require Import riscv.Utility.Monads.
+Require Import riscv.Utility.MonadNotations.
+Require Export riscv.Utility.FreeMonad.
+Require Import riscv.Spec.Decode.
+Require Import riscv.Spec.Machine.
+Require Import riscv.Utility.Utility.
+Require Import riscv.Spec.Primitives.
+Require Import Coq.Lists.List. Import ListNotations.
+Require Import coqutil.Datatypes.List.
+Require Import coqutil.Datatypes.ListSet.
+Require Export riscv.Platform.RiscvMachine.
+Require Export riscv.Platform.MaterializeRiscvProgram.
+Require Import coqutil.Z.Lia.
+Require Import coqutil.Map.Interface.
+Require Import coqutil.Map.Properties.
+Require Import coqutil.Datatypes.PropSet.
+Require Import coqutil.Tactics.Tactics.
+Require Import riscv.Platform.Sane.
+
+Local Open Scope Z_scope.
+Local Open Scope bool_scope.
+
+Class MMIOSpec{W: Words} {Mem : map.map word byte} := {
+  (* should not say anything about alignment, just whether it's in the MMIO range *)
+  isMMIOAddr: word -> Prop;
+
+  (* alignment and load size checks *)
+  isMMIOAligned: nat -> word -> Prop;
+
+  (* hardware guarantees on MMIO read values *)
+  MMIOReadOK : nat -> list LogItem -> word -> word -> Prop;
+}.
+
+Definition natToStr(n: nat): string := DecimalString.NilZero.string_of_uint (Nat.to_uint n).
+
+Section Riscv.
+  Import free.
+  Context {W: Words} {Mem: map.map word byte} {Registers: map.map Register word}.
+
+  Definition mmioLoadEvent(addr: word){n: nat}(v: HList.tuple byte n): LogItem :=
+    ((map.empty, ("MMIOREAD" ++ natToStr (8 * n))%string, [addr]),
+     (map.empty, [word.of_Z (LittleEndian.combine n v)])).
+
+  Definition mmioStoreEvent(addr: word){n: nat}(v: HList.tuple byte n): LogItem :=
+    ((map.empty, ("MMIOWRITE" ++ natToStr (8 * n))%string,
+      [addr; word.of_Z (LittleEndian.combine n v)]), (map.empty, [])).
+
+  Context {mmio_spec: MMIOSpec}.
+
+  Definition nonmem_store(n: nat)(ctxid: SourceType) a v mach post :=
+    isMMIOAddr a /\ isMMIOAligned n a /\
+    post (withXAddrs (invalidateWrittenXAddrs n a mach.(getXAddrs))
+         (withLogItem (@mmioStoreEvent a n v)
+         mach)).
+
+  Definition store(n: nat)(ctxid: SourceType) a v mach post :=
+    match Memory.store_bytes n mach.(getMem) a v with
+    | Some m => post (withXAddrs (invalidateWrittenXAddrs n a mach.(getXAddrs)) (withMem m mach))
+    | None => nonmem_store n ctxid a v mach post
+    end.
+
+  Definition nonmem_load(n: nat)(ctxid: SourceType) a mach (post: _ -> _ -> Prop) :=
+    isMMIOAddr a /\ isMMIOAligned n a
+    (* there exists at least one valid MMIO read value (set is nonempty) *)
+    /\ (exists v, MMIOReadOK n (getLog mach) a (word.of_Z (LittleEndian.combine n v)))
+    (* ...and postcondition holds for all valid read values *)
+    /\ forall v,
+        MMIOReadOK n (getLog mach) a (word.of_Z (LittleEndian.combine n v)) ->
+        post v (withLogItem (@mmioLoadEvent a n v) mach).
+
+  Definition load(n: nat)(ctxid: SourceType) a mach post :=
+    (ctxid = Fetch -> isXAddr4 a mach.(getXAddrs)) /\
+    match Memory.load_bytes n mach.(getMem) a with
+    | Some v => post v mach
+    | None => nonmem_load n ctxid a mach post
+    end.
+
+  Definition updatePc(mach: RiscvMachine): RiscvMachine :=
+    withPc mach.(getNextPc) (withNextPc (word.add mach.(getNextPc) (word.of_Z 4)) mach).
+
+  Definition interpret_action (a : riscv_primitive) (mach : RiscvMachine) :
+    (primitive_result a -> RiscvMachine -> Prop) -> (RiscvMachine -> Prop) -> Prop :=
+    match a with
+    | GetRegister reg => fun (postF: word -> RiscvMachine -> Prop) postA =>
+        let v :=
+          if Z.eq_dec reg 0 then word.of_Z 0
+          else match map.get mach.(getRegs) reg with
+               | Some x => x
+               | None => word.of_Z 0 end in
+        postF v mach
+    | SetRegister reg v => fun postF postA =>
+      let regs := if Z.eq_dec reg Register0
+                  then mach.(getRegs)
+                  else map.put mach.(getRegs) reg v in
+      postF tt (withRegs regs mach)
+    | GetPC => fun postF postA => postF mach.(getPc) mach
+    | SetPC newPC => fun postF postA => postF tt (withNextPc newPC mach)
+    | LoadByte ctxid a => fun postF postA => load 1 ctxid a mach postF
+    | LoadHalf ctxid a => fun postF postA => load 2 ctxid a mach postF
+    | LoadWord ctxid a => fun postF postA => load 4 ctxid a mach postF
+    | LoadDouble ctxid a => fun postF postA => load 8 ctxid a mach postF
+    | StoreByte ctxid a v => fun postF postA => store 1 ctxid a v mach (postF tt)
+    | StoreHalf ctxid a v => fun postF postA => store 2 ctxid a v mach (postF tt)
+    | StoreWord ctxid a v => fun postF postA => store 4 ctxid a v mach (postF tt)
+    | StoreDouble ctxid a v => fun postF postA => store 8 ctxid a v mach (postF tt)
+    | EndCycleNormal => fun postF postA => postF tt (updatePc mach)
+    | EndCycleEarly _ => fun postF postA => postA (updatePc mach) (* ignores postF containing the continuation *)
+    | MakeReservation _
+    | ClearReservation _
+    | CheckReservation _
+    | GetCSRField _
+    | SetCSRField _ _
+    | GetPrivMode
+    | SetPrivMode _
+    | Fence _ _
+        => fun postF postA => False
+    end.
+
+  Definition MinimalMMIOPrimitivesParams:
+    PrimitivesParams (free riscv_primitive primitive_result) RiscvMachine :=
+  {|
+    Primitives.mcomp_sat A m mach postF :=
+      @free.interpret _ _ _ interpret_action A m mach postF (fun _ => False);
+    Primitives.is_initial_register_value x := True;
+    Primitives.nonmem_load := nonmem_load;
+    Primitives.nonmem_store := nonmem_store;
+    Primitives.valid_machine mach :=
+      map.undef_on mach.(getMem) isMMIOAddr /\ disjoint (of_list mach.(getXAddrs)) isMMIOAddr;
+  |}.
+
+  Lemma load_weaken_post n c a m (post1 post2:_->_->Prop)
+    (H: forall r s, post1 r s -> post2 r s)
+    : load n c a m post1 -> load n c a m post2.
+  Proof.
+    cbv [load nonmem_load].
+    destruct (Memory.load_bytes n (getMem m) a); intuition eauto.
+  Qed.
+
+  Lemma store_weaken_post n c a v m (post1 post2:_->Prop)
+    (H: forall s, post1 s -> post2 s)
+    : store n c a v m post1 -> store n c a v m post2.
+  Proof.
+    cbv [store nonmem_store].
+    destruct (Memory.store_bytes n (getMem m) a); intuition eauto.
+  Qed.
+
+  Lemma interpret_action_weaken_post a (postF1 postF2: _ -> _ -> Prop) (postA1 postA2: _ -> Prop):
+    (forall r s, postF1 r s -> postF2 r s) ->
+    (forall s, postA1 s -> postA2 s) ->
+    forall s, interpret_action a s postF1 postA1 -> interpret_action a s postF2 postA2.
+  Proof.
+    destruct a; cbn; try solve [intuition eauto].
+    all : eauto using load_weaken_post, store_weaken_post.
+  Qed.
+
+  Global Instance MinimalMMIOSatisfies_mcomp_sat_spec: mcomp_sat_spec MinimalMMIOPrimitivesParams.
+  Proof.
+    split; cbv [mcomp_sat MinimalMMIOPrimitivesParams Bind Return Monad_free].
+    { symmetry. eapply interpret_bind_ex_mid, interpret_action_weaken_post. }
+    { symmetry; intros. rewrite interpret_ret; eapply iff_refl. }
+  Qed.
+
+  Lemma preserve_undef_on{memOk: map.ok Mem}: forall n (m m': Mem) a w s,
+      Memory.store_bytes n m a w = Some m' ->
+      map.undef_on m s ->
+      map.undef_on m' s.
+  Proof.
+    eauto using map.same_domain_preserves_undef_on, Memory.store_bytes_preserves_domain.
+  Qed.
+
+  Lemma interpret_action_total{memOk: map.ok Mem} a s postF postA :
+    map.undef_on s.(getMem) isMMIOAddr ->
+    disjoint (of_list s.(getXAddrs)) isMMIOAddr ->
+    interpret_action a s postF postA ->
+    exists s', map.undef_on s'.(getMem) isMMIOAddr /\
+          disjoint (of_list s'.(getXAddrs)) isMMIOAddr /\
+          (postA s' \/ exists v', postF v' s').
+  Proof.
+    destruct s, a; cbn -[HList.tuple];
+      cbv [load store nonmem_load nonmem_store]; cbn -[HList.tuple];
+        repeat destruct_one_match;
+        intuition idtac;
+        repeat lazymatch goal with
+               | H : postF _ ?mach |- exists _ : RiscvMachine, _ =>
+                 exists mach; cbn [RiscvMachine.getMem RiscvMachine.getXAddrs]
+               | H : postA ?mach |- exists _ : RiscvMachine, _ =>
+                 exists mach; cbn [RiscvMachine.getMem RiscvMachine.getXAddrs]
+               | Hexists : (exists v, ?P), Hforall : (forall v, ?P -> _) |- _ =>
+                 let v := fresh "v" in
+                 destruct Hexists as [v Hexists];
+                   specialize (Hforall v Hexists)
+               end;
+        ssplit; eauto; simpl;
+        change removeXAddr with (@List.removeb word word.eqb _);
+        rewrite ?ListSet.of_list_removeb;
+        intuition eauto 10 using preserve_undef_on, disjoint_diff_l.
+  Qed.
+
+  Lemma interpret_action_total'{memOk: map.ok Mem} a s post :
+    map.undef_on s.(getMem) isMMIOAddr ->
+    disjoint (of_list s.(getXAddrs)) isMMIOAddr ->
+    interpret_action a s post (fun _ : RiscvMachine => False) ->
+    exists v s', post v s' /\ map.undef_on s'.(getMem) isMMIOAddr
+                           /\ disjoint (of_list s'.(getXAddrs)) isMMIOAddr.
+  Proof.
+    intros. pose proof interpret_action_total as P.
+    specialize P with (postA := (fun _ : RiscvMachine => False)). simpl in P.
+    specialize (P _ _ _ H H0 H1).
+    destruct P as (s' & ? & ? & ?).
+    destruct H4 as [[] | (v' & ?)].
+    eauto.
+  Qed.
+
+  Import coqutil.Tactics.Tactics.
+
+  Lemma interpret_action_appendonly a s postF postA :
+    interpret_action a s postF postA ->
+    interpret_action a s (fun _ s' => endswith s'.(getLog) s.(getLog))
+                           (fun s' => endswith s'.(getLog) s.(getLog)).
+  Proof.
+    destruct s, a; cbn; cbv [load store nonmem_load nonmem_store]; cbn;
+      repeat destruct_one_match;
+      intuition eauto using endswith_refl, endswith_cons_l.
+  Qed.
+
+  (* NOTE: maybe instead a generic lemma to push /\ into postcondition? *)
+  Lemma interpret_action_appendonly' a s postF postA :
+    interpret_action a s postF postA ->
+    interpret_action a s (fun v s' => postF v s' /\ endswith s'.(getLog) s.(getLog))
+                         (fun   s' => postA   s' /\ endswith s'.(getLog) s.(getLog)).
+  Proof.
+    destruct s, a; cbn; cbv [load store nonmem_load nonmem_store]; cbn;
+      repeat destruct_one_match; intros; destruct_products; try split;
+        intuition eauto using endswith_refl, endswith_cons_l.
+  Qed.
+
+  Lemma interpret_action_appendonly'' a s post :
+    interpret_action a s post (fun _ : RiscvMachine => False) ->
+    interpret_action a s (fun v s' => post v s' /\ endswith s'.(getLog) s.(getLog))
+                         (fun _ : RiscvMachine => False).
+  Proof.
+    intros. pose proof interpret_action_appendonly' as P.
+    specialize (P _ _ _ (fun _ : RiscvMachine => False) H). simpl in P.
+    eapply interpret_action_weaken_post. 3: exact P. all: simpl; intuition eauto.
+  Qed.
+
+  Lemma interpret_action_preserves_valid{memOk: map.ok Mem} a s postF postA :
+    map.undef_on s.(getMem) isMMIOAddr ->
+    disjoint (of_list s.(getXAddrs)) isMMIOAddr ->
+    interpret_action a s postF postA ->
+    interpret_action a s (fun v s' => postF v s' /\
+                                      map.undef_on s'.(getMem) isMMIOAddr /\
+                                      disjoint (of_list s'.(getXAddrs)) isMMIOAddr)
+                         (fun s' => postA s' /\
+                                    map.undef_on s'.(getMem) isMMIOAddr /\
+                                    disjoint (of_list s'.(getXAddrs)) isMMIOAddr).
+  Proof.
+    destruct s, a; cbn; cbv [load store nonmem_load nonmem_store]; cbn;
+      repeat destruct_one_match; intros; destruct_products; try split;
+        change removeXAddr with (@List.removeb word word.eqb _);
+        rewrite ?ListSet.of_list_removeb;
+        intuition eauto 10 using preserve_undef_on, disjoint_diff_l.
+  Qed.
+
+  Lemma interpret_action_preserves_valid'{memOk: map.ok Mem} a s post :
+    map.undef_on s.(getMem) isMMIOAddr ->
+    disjoint (of_list s.(getXAddrs)) isMMIOAddr ->
+    interpret_action a s post (fun _ : RiscvMachine => False) ->
+    interpret_action a s (fun v s' => post v s' /\ map.undef_on s'.(getMem) isMMIOAddr /\
+                                      disjoint (of_list s'.(getXAddrs)) isMMIOAddr)
+                         (fun _ : RiscvMachine => False).
+  Proof.
+    intros. pose proof interpret_action_preserves_valid as P.
+    specialize (P _ _ _ (fun _ : RiscvMachine => False) H H0 H1). simpl in P.
+    eapply interpret_action_weaken_post. 3: exact P. all: simpl; intuition eauto.
+  Qed.
+
+  Global Instance MinimalMMIOPrimitivesSane{memOk: map.ok Mem} :
+    PrimitivesSane MinimalMMIOPrimitivesParams.
+  Proof.
+    split; cbv [mcomp_sane valid_machine MinimalMMIOPrimitivesParams]; intros *; intros [U D] M;
+      (split; [ exact (interpret_action_total' _ st _ U D M)
+              | eapply interpret_action_preserves_valid'; try eassumption;
+                eapply interpret_action_appendonly''; try eassumption ]).
+  Qed.
+
+  Global Instance MinimalMMIOSatisfiesPrimitives{memOk: map.ok Mem} :
+    Primitives MinimalMMIOPrimitivesParams.
+  Proof.
+    split; try exact _.
+    all : cbv [mcomp_sat spec_load spec_store MinimalMMIOPrimitivesParams invalidateWrittenXAddrs].
+    all: intros;
+      repeat match goal with
+      | _ => progress subst
+      | _ => Option.inversion_option
+      | _ => progress cbn -[Memory.load_bytes Memory.store_bytes HList.tuple]
+      | _ => progress cbv [valid_register is_initial_register_value load store Memory.loadByte Memory.loadHalf Memory.loadWord Memory.loadDouble Memory.storeByte Memory.storeHalf Memory.storeWord Memory.storeDouble] in *
+      | H : exists _, _ |- _ => destruct H
+      | H : _ /\ _ |- _ => destruct H
+      | |- _ => solve [ intuition (eauto || blia) ]
+      | H : _ \/ _ |- _ => destruct H
+      | |- context[match ?x with _ => _ end] => destruct x eqn:?
+      | |-_ /\ _ => split
+      end.
+      (* setRegister *)
+      destruct initialL; eassumption.
+  Qed.
+
+End Riscv.
